tests/lean/run/premise_selection_mepo.lean
@@ -1,6 +1,17 @@
 import Lean.PremiseSelection.MePo
 
-set_premise_selector Lean.PremiseSelection.mepo
+set_premise_selector fun g _ => Lean.PremiseSelection.mepo (useRarity := false) g
+
+example (a b : Int) : a + b = b + a := by
+  suggest_premises
+  sorry
+
+#time
+example (x y z : List Int) : x ++ y ++ z = x ++ (y ++ z) := by
+  suggest_premises
+  sorry
+
+set_premise_selector fun g _ => Lean.PremiseSelection.mepo (useRarity := true) g
 
 example (a b : Int) : a + b = b + a := by
   suggest_premises
